test/ExtendedArbitraries/Identifiers.dfy
@@ -1,0 +1,28 @@
+include "../../src/ExtendedArbitraries/Identifiers.dfy"
+include "../../src/RandomGenerator.dfy"
+
+module ExtIdentifiersTest {
+  import opened Arbitrary
+  import opened RandomGenerator
+  import opened ExtIdentifiers
+
+  method {:test} TestUUID() {
+    var arb := UUID();
+    var rng := XoroShift128Plus.fromSeed(42);
+    var tc := new TestCase([], rng, 100, true);
+    var res := arb.Apply(tc);
+    // 8-4-4-4-12 layout: 32 hex digits + 4 dashes = 36 chars, dashes fixed.
+    expect |res| == 36;
+    expect res[8] == '-' && res[13] == '-' && res[18] == '-' && res[23] == '-';
+    print "UUID: ", res, "\n";
+  }
+
+  method {:test} TestULID() {
+    var arb := ULID();
+    var rng := XoroShift128Plus.fromSeed(42);
+    var tc := new TestCase([], rng, 100, true);
+    var res := arb.Apply(tc);
+    expect |res| == 26;
+    print "ULID: ", res, "\n";
+  }
+}
