test/ExtendedArbitraries/Json.dfy
@@ -1,0 +1,17 @@
+include "../../src/ExtendedArbitraries/Json.dfy"
+include "../../src/RandomGenerator.dfy"
+
+module ExtJsonTest {
+  import opened Arbitrary
+  import opened RandomGenerator
+  import opened ExtJson
+
+  method {:test} TestJson() {
+    var arb := Json();
+    var rng := XoroShift128Plus.fromSeed(42);
+    var tc := new TestCase([], rng, 100, true);
+    var res := arb.Apply(tc);
+    expect |res| >= 1;
+    print "Json: ", res, "\n";
+  }
+}
