test/ExtendedArbitraries/Network.dfy
@@ -1,0 +1,26 @@
+include "../../src/ExtendedArbitraries/Network.dfy"
+include "../../src/RandomGenerator.dfy"
+
+module ExtNetworkTest {
+  import opened Arbitrary
+  import opened RandomGenerator
+  import opened ExtNetwork
+
+  method {:test} TestIPv4() {
+    var arb := IPv4();
+    var rng := XoroShift128Plus.fromSeed(42);
+    var tc := new TestCase([], rng, 100, true);
+    var res := arb.Apply(tc);
+    expect '.' in res;
+    print "IPv4: ", res, "\n";
+  }
+
+  method {:test} TestIPv6() {
+    var arb := IPv6();
+    var rng := XoroShift128Plus.fromSeed(42);
+    var tc := new TestCase([], rng, 100, true);
+    var res := arb.Apply(tc);
+    expect ':' in res;
+    print "IPv6: ", res, "\n";
+  }
+}
