test/ExtendedArbitraries/Web.dfy
@@ -1,0 +1,26 @@
+include "../../src/ExtendedArbitraries/Web.dfy"
+include "../../src/RandomGenerator.dfy"
+
+module ExtWebTest {
+  import opened Arbitrary
+  import opened RandomGenerator
+  import opened ExtWeb
+
+  method {:test} TestDomain() {
+    var arb := Domain();
+    var rng := XoroShift128Plus.fromSeed(42);
+    var tc := new TestCase([], rng, 100, true);
+    var res := arb.Apply(tc);
+    expect '.' in res;
+    print "Domain: ", res, "\n";
+  }
+
+  method {:test} TestEmail() {
+    var arb := Email();
+    var rng := XoroShift128Plus.fromSeed(42);
+    var tc := new TestCase([], rng, 100, true);
+    var res := arb.Apply(tc);
+    expect '@' in res;
+    print "Email: ", res, "\n";
+  }
+}
